p256: mv fromDomain to Hacl.Impl.P256.Field

code/ecdsap256/Hacl.Impl.P256.Core.fst
@@ -34,16 +34,3 @@ let toDomain f res =
   bn_lshift256 f multBuffer;
   solinas_reduction_impl multBuffer res;
   pop_frame()
-
-
-
-// TODO: mv to Hacl.Impl.P256.Field
-inline_for_extraction noextract
-val fromDomain: f:felem -> res:felem -> Stack unit
-  (requires fun h -> live h f /\ live h res /\ as_nat h f < S.prime)
-  (ensures fun h0 _ h1 -> modifies (loc res) h0 h1 /\
-    as_nat h1 res = (as_nat h0 f * mont_R_inv) % S.prime /\
-    as_nat h1 res = fromDomain_ (as_nat h0 f))
-
-let fromDomain f res =
-  montgomery_multiplication_buffer_by_one f res
